README.md
@@ -16,13 +16,12 @@ Volume 7 Issue 6, November 1997, 661 - 666
 
 TODO:
 - size_diff (redo with Racket generation, big_oh)   [robby]
-- make_array_td (big_oh) [robby]
 - make_array_bu (time, correctness, extraction, big_oh) [max]
 - to_list_naive (exact time [vs bound], big_oh)
 - to_list_bu (time, correctness, extraction, big_oh)
 - investigate sub1's running time (should we consider it constant?)
 - improve coq parser and use it everywhere [robby]
-- rearrange the files & directories in the repo [robby]
-- move the rest of the files out of tmonad/ into function-specific directories
+- move the rest of the files out of tmonad/ into function-specific directories [robby]
 - rename the files in rkt/ to match the new naming convention (the
-  function name followed by the running time)
+  function name followed by the running time) [robby]
+
